- fix up to prop_basic

proof/old_system/uni/def_ott.v
@@ -140,19 +140,19 @@ with open_body_wrt_exp_rec (k:nat) (e5:exp) (body5:body) : body :=
   | (body_anno e A) => body_anno (open_exp_wrt_exp_rec k e5 e) A
 end.
 
-Fixpoint open_contd_wrt_typ_rec (k:nat) (A5:typ) (cd5:contd) {struct cd5}: contd :=
-  match cd5 with
-  | (contd_infabsunion A cd) => contd_infabsunion (open_typ_wrt_typ_rec k A5 A) (open_contd_wrt_typ_rec k A5 cd)
-  | (contd_infapp e cs) => contd_infapp (open_exp_wrt_typ_rec k A5 e) (open_conts_wrt_typ_rec k A5 cs)
-  | (contd_unioninfabs A B cd) => contd_unioninfabs (open_typ_wrt_typ_rec k A5 A) (open_typ_wrt_typ_rec k A5 B) (open_contd_wrt_typ_rec k A5 cd)
-end
-with open_conts_wrt_typ_rec (k:nat) (A_5:typ) (cs5:conts) {struct cs5}: conts :=
+Fixpoint open_conts_wrt_typ_rec (k:nat) (A_5:typ) (cs5:conts) {struct cs5}: conts :=
   match cs5 with
   | (conts_infabs cd) => conts_infabs (open_contd_wrt_typ_rec k A_5 cd)
   | (conts_inftapp A cs) => conts_inftapp (open_typ_wrt_typ_rec k A_5 A) (open_conts_wrt_typ_rec k A_5 cs)
   | (conts_inftappunion A1 A2 cs) => conts_inftappunion (open_typ_wrt_typ_rec k A_5 A1) (open_typ_wrt_typ_rec k A_5 A2) (open_conts_wrt_typ_rec k A_5 cs)
   | (conts_unioninftapp A2 cs) => conts_unioninftapp (open_typ_wrt_typ_rec k A_5 A2) (open_conts_wrt_typ_rec k A_5 cs)
   | (conts_sub A) => conts_sub (open_typ_wrt_typ_rec k A_5 A)
+end
+with open_contd_wrt_typ_rec (k:nat) (A5:typ) (cd5:contd) {struct cd5}: contd :=
+  match cd5 with
+  | (contd_infabsunion A cd) => contd_infabsunion (open_typ_wrt_typ_rec k A5 A) (open_contd_wrt_typ_rec k A5 cd)
+  | (contd_infapp e cs) => contd_infapp (open_exp_wrt_typ_rec k A5 e) (open_conts_wrt_typ_rec k A5 cs)
+  | (contd_unioninfabs A B cd) => contd_unioninfabs (open_typ_wrt_typ_rec k A5 A) (open_typ_wrt_typ_rec k A5 B) (open_contd_wrt_typ_rec k A5 cd)
 end.
 
 Fixpoint open_contd_wrt_exp_rec (k:nat) (e5:exp) (cd5:contd) {struct cd5}: contd :=
@@ -168,13 +168,6 @@ with open_conts_wrt_exp_rec (k:nat) (e5:exp) (cs5:conts) {struct cs5}: conts :=
   | (conts_inftappunion A1 A2 cs) => conts_inftappunion A1 A2 (open_conts_wrt_exp_rec k e5 cs)
   | (conts_unioninftapp A2 cs) => conts_unioninftapp A2 (open_conts_wrt_exp_rec k e5 cs)
   | (conts_sub A) => conts_sub A
-end.
-
-Definition open_dbind_wrt_typ_rec (k:nat) (A5:typ) (db5:dbind) : dbind :=
-  match db5 with
-  | dbind_tvar_empty => dbind_tvar_empty 
-  | dbind_stvar_empty => dbind_stvar_empty 
-  | (dbind_typ A) => dbind_typ (open_typ_wrt_typ_rec k A5 A)
 end.
 
 Definition open_work_wrt_typ_rec (k:nat) (A_5:typ) (w5:work) : work :=
@@ -193,6 +186,14 @@ Definition open_work_wrt_typ_rec (k:nat) (A_5:typ) (w5:work) : work :=
   | (work_applyd cd A B) => work_applyd (open_contd_wrt_typ_rec k A_5 cd) (open_typ_wrt_typ_rec k A_5 A) (open_typ_wrt_typ_rec k A_5 B)
 end.
 
+Definition open_abind_wrt_typ_rec (k:nat) (A5:typ) (ab5:abind) : abind :=
+  match ab5 with
+  | abind_tvar_empty => abind_tvar_empty 
+  | abind_stvar_empty => abind_stvar_empty 
+  | abind_etvar_empty => abind_etvar_empty 
+  | (abind_var_typ A) => abind_var_typ (open_typ_wrt_typ_rec k A5 A)
+end.
+
 Definition open_work_wrt_exp_rec (k:nat) (e5:exp) (w5:work) : work :=
   match w5 with
   | (work_infer e cs) => work_infer (open_exp_wrt_exp_rec k e5 e) (open_conts_wrt_exp_rec k e5 cs)
@@ -209,33 +210,11 @@ Definition open_work_wrt_exp_rec (k:nat) (e5:exp) (w5:work) : work :=
   | (work_applyd cd A B) => work_applyd (open_contd_wrt_exp_rec k e5 cd) A B
 end.
 
-Definition open_abind_wrt_typ_rec (k:nat) (A5:typ) (ab5:abind) : abind :=
-  match ab5 with
-  | abind_tvar_empty => abind_tvar_empty 
-  | abind_stvar_empty => abind_stvar_empty 
-  | abind_etvar_empty => abind_etvar_empty 
-  | (abind_var_typ A) => abind_var_typ (open_typ_wrt_typ_rec k A5 A)
-end.
-
-Fixpoint open_dworklist_wrt_typ_rec (k:nat) (A5:typ) (Ω5:dworklist) {struct Ω5}: dworklist :=
-  match Ω5 with
-  | dworklist_empty => dworklist_empty 
-  | (dworklist_cons_var Ω X db) => dworklist_cons_var (open_dworklist_wrt_typ_rec k A5 Ω) X (open_dbind_wrt_typ_rec k A5 db)
-  | (dworklist_cons_work Ω w) => dworklist_cons_work (open_dworklist_wrt_typ_rec k A5 Ω) (open_work_wrt_typ_rec k A5 w)
-end.
-
-Fixpoint open_dworklist_wrt_exp_rec (k:nat) (e5:exp) (Ω5:dworklist) {struct Ω5}: dworklist :=
-  match Ω5 with
-  | dworklist_empty => dworklist_empty 
-  | (dworklist_cons_var Ω X db) => dworklist_cons_var (open_dworklist_wrt_exp_rec k e5 Ω) X db
-  | (dworklist_cons_work Ω w) => dworklist_cons_work (open_dworklist_wrt_exp_rec k e5 Ω) (open_work_wrt_exp_rec k e5 w)
-end.
-
-Fixpoint open_aworklist_wrt_exp_rec (k:nat) (e5:exp) (Γ_5:aworklist) {struct Γ_5}: aworklist :=
-  match Γ_5 with
-  | aworklist_empty => aworklist_empty 
-  | (aworklist_cons_var Γ X ab) => aworklist_cons_var (open_aworklist_wrt_exp_rec k e5 Γ) X ab
-  | (aworklist_cons_work Γ w) => aworklist_cons_work (open_aworklist_wrt_exp_rec k e5 Γ) (open_work_wrt_exp_rec k e5 w)
+Definition open_dbind_wrt_typ_rec (k:nat) (A5:typ) (db5:dbind) : dbind :=
+  match db5 with
+  | dbind_tvar_empty => dbind_tvar_empty 
+  | dbind_stvar_empty => dbind_stvar_empty 
+  | (dbind_typ A) => dbind_typ (open_typ_wrt_typ_rec k A5 A)
 end.
 
 Fixpoint open_aworklist_wrt_typ_rec (k:nat) (A5:typ) (Γ_5:aworklist) {struct Γ_5}: aworklist :=
@@ -245,39 +224,60 @@ Fixpoint open_aworklist_wrt_typ_rec (k:nat) (A5:typ) (Γ_5:aworklist) {struct Γ
   | (aworklist_cons_work Γ w) => aworklist_cons_work (open_aworklist_wrt_typ_rec k A5 Γ) (open_work_wrt_typ_rec k A5 w)
 end.
 
-Definition open_exp_wrt_typ A_5 e_5 := open_exp_wrt_typ_rec 0 e_5 A_5.
+Fixpoint open_aworklist_wrt_exp_rec (k:nat) (e5:exp) (Γ_5:aworklist) {struct Γ_5}: aworklist :=
+  match Γ_5 with
+  | aworklist_empty => aworklist_empty 
+  | (aworklist_cons_var Γ X ab) => aworklist_cons_var (open_aworklist_wrt_exp_rec k e5 Γ) X ab
+  | (aworklist_cons_work Γ w) => aworklist_cons_work (open_aworklist_wrt_exp_rec k e5 Γ) (open_work_wrt_exp_rec k e5 w)
+end.
 
-Definition open_work_wrt_exp e5 w5 := open_work_wrt_exp_rec 0 w5 e5.
+Fixpoint open_dworklist_wrt_exp_rec (k:nat) (e5:exp) (Ω5:dworklist) {struct Ω5}: dworklist :=
+  match Ω5 with
+  | dworklist_empty => dworklist_empty 
+  | (dworklist_cons_var Ω X db) => dworklist_cons_var (open_dworklist_wrt_exp_rec k e5 Ω) X db
+  | (dworklist_cons_work Ω w) => dworklist_cons_work (open_dworklist_wrt_exp_rec k e5 Ω) (open_work_wrt_exp_rec k e5 w)
+end.
+
+Fixpoint open_dworklist_wrt_typ_rec (k:nat) (A5:typ) (Ω5:dworklist) {struct Ω5}: dworklist :=
+  match Ω5 with
+  | dworklist_empty => dworklist_empty 
+  | (dworklist_cons_var Ω X db) => dworklist_cons_var (open_dworklist_wrt_typ_rec k A5 Ω) X (open_dbind_wrt_typ_rec k A5 db)
+  | (dworklist_cons_work Ω w) => dworklist_cons_work (open_dworklist_wrt_typ_rec k A5 Ω) (open_work_wrt_typ_rec k A5 w)
+end.
+
+Definition open_aworklist_wrt_typ A5 Γ_5 := open_aworklist_wrt_typ_rec 0 Γ_5 A5.
+
+Definition open_abind_wrt_typ A5 ab5 := open_abind_wrt_typ_rec 0 ab5 A5.
+
+Definition open_contd_wrt_typ A5 cd5 := open_contd_wrt_typ_rec 0 cd5 A5.
 
 Definition open_work_wrt_typ A_5 w5 := open_work_wrt_typ_rec 0 w5 A_5.
 
 Definition open_dbind_wrt_typ A5 db5 := open_dbind_wrt_typ_rec 0 db5 A5.
 
-Definition open_contd_wrt_exp e5 cd5 := open_contd_wrt_exp_rec 0 cd5 e5.
-
-Definition open_dworklist_wrt_typ A5 Ω5 := open_dworklist_wrt_typ_rec 0 Ω5 A5.
-
-Definition open_typ_wrt_typ A_5 A__6 := open_typ_wrt_typ_rec 0 A__6 A_5.
-
-Definition open_body_wrt_exp e5 body5 := open_body_wrt_exp_rec 0 body5 e5.
-
-Definition open_dworklist_wrt_exp e5 Ω5 := open_dworklist_wrt_exp_rec 0 Ω5 e5.
-
-Definition open_contd_wrt_typ A5 cd5 := open_contd_wrt_typ_rec 0 cd5 A5.
+Definition open_aworklist_wrt_exp e5 Γ_5 := open_aworklist_wrt_exp_rec 0 Γ_5 e5.
 
 Definition open_exp_wrt_exp e_5 e__6 := open_exp_wrt_exp_rec 0 e__6 e_5.
 
-Definition open_conts_wrt_typ A_5 cs5 := open_conts_wrt_typ_rec 0 cs5 A_5.
-
-Definition open_aworklist_wrt_exp e5 Γ_5 := open_aworklist_wrt_exp_rec 0 Γ_5 e5.
-
-Definition open_abind_wrt_typ A5 ab5 := open_abind_wrt_typ_rec 0 ab5 A5.
-
-Definition open_aworklist_wrt_typ A5 Γ_5 := open_aworklist_wrt_typ_rec 0 Γ_5 A5.
-
 Definition open_conts_wrt_exp e5 cs5 := open_conts_wrt_exp_rec 0 cs5 e5.
 
+Definition open_dworklist_wrt_exp e5 Ω5 := open_dworklist_wrt_exp_rec 0 Ω5 e5.
+
+Definition open_exp_wrt_typ A_5 e_5 := open_exp_wrt_typ_rec 0 e_5 A_5.
+
 Definition open_body_wrt_typ A5 body5 := open_body_wrt_typ_rec 0 body5 A5.
+
+Definition open_conts_wrt_typ A_5 cs5 := open_conts_wrt_typ_rec 0 cs5 A_5.
+
+Definition open_typ_wrt_typ A_5 A__6 := open_typ_wrt_typ_rec 0 A__6 A_5.
+
+Definition open_contd_wrt_exp e5 cd5 := open_contd_wrt_exp_rec 0 cd5 e5.
+
+Definition open_work_wrt_exp e5 w5 := open_work_wrt_exp_rec 0 w5 e5.
+
+Definition open_dworklist_wrt_typ A5 Ω5 := open_dworklist_wrt_typ_rec 0 Ω5 A5.
+
+Definition open_body_wrt_exp e5 body5 := open_body_wrt_exp_rec 0 body5 e5.
 
 (** closing up abstractions *)
 Fixpoint close_typ_wrt_typ_rec (k:nat) (A_5:var) (A__6:typ) {struct A__6}: typ :=
@@ -1161,7 +1161,6 @@ Inductive d_wf_typ : denv -> typ -> Prop :=    (* defn d_wf_typ *)
      d_wf_typ Ψ A2 ->
      d_wf_typ Ψ (typ_arrow A1 A2)
  | d_wf_typ__all : forall (L:vars) (Ψ:denv) (A:typ),
-      ( forall X , X \notin  L  -> s_in X  ( open_typ_wrt_typ A (typ_var_f X) )  )  ->
       ( forall X , X \notin  L  -> d_wf_typ  ( X ~ dbind_tvar_empty  ++  Ψ )   ( open_typ_wrt_typ A (typ_var_f X) )  )  ->
      d_wf_typ Ψ (typ_all A)
  | d_wf_typ__union : forall (Ψ:denv) (A1 A2:typ),
@@ -1189,7 +1188,6 @@ Inductive d_wf_exp : denv -> exp -> Prop :=    (* defn d_wf_exp *)
      d_wf_exp Ψ e2 ->
      d_wf_exp Ψ (exp_app e1 e2)
  | d_wf_exp__tabs : forall (L:vars) (Ψ:denv) (body5:body),
-      ( forall X , X \notin  L  -> s_in_b X  ( open_body_wrt_typ body5 (typ_var_f X) )  )  ->
       ( forall X , X \notin  L  -> d_wf_body  ( X ~ dbind_tvar_empty  ++  Ψ )   ( open_body_wrt_typ body5 (typ_var_f X) )  )  ->
      d_wf_exp Ψ (exp_tabs body5)
  | d_wf_exp__tapp : forall (Ψ:denv) (e:exp) (A:typ),
@@ -1370,6 +1368,33 @@ Inductive d_wf_wl : dworklist -> Prop :=    (* defn d_wf_wl *)
      d_wf_wl Ω ->
      d_wf_wl (dworklist_cons_work Ω (work_sub A B)).
 
+(* defns J_strong_neq_stvar *)
+Inductive s_neq_stvar : denv -> typ -> Prop :=    (* defn s_neq_stvar *)
+ | s_neq_stvar__unit : forall (Ψ:denv),
+     s_neq_stvar Ψ typ_unit
+ | s_neq_stvar__top : forall (Ψ:denv),
+     s_neq_stvar Ψ typ_top
+ | s_neq_stvar__bot : forall (Ψ:denv),
+     s_neq_stvar Ψ typ_bot
+ | s_neq_stvar__tvar : forall (Ψ:denv) (X:typvar),
+      binds ( X )  ( dbind_tvar_empty ) ( Ψ )  ->
+     s_neq_stvar Ψ (typ_var_f X)
+ | s_neq_stvar__arrow : forall (Ψ:denv) (A1 A2:typ),
+     lc_typ A1 ->
+     lc_typ A2 ->
+     s_neq_stvar Ψ (typ_arrow A1 A2)
+ | s_neq_stvar__all : forall (Ψ:denv) (A:typ),
+     lc_typ (typ_all A) ->
+     s_neq_stvar Ψ (typ_all A)
+ | s_neq_stvar__union : forall (Ψ:denv) (A1 A2:typ),
+     s_neq_stvar Ψ A1 ->
+     s_neq_stvar Ψ A2 ->
+     s_neq_stvar Ψ (typ_union A1 A2)
+ | s_neq_stvar__intersection : forall (Ψ:denv) (A1 A2:typ),
+     s_neq_stvar Ψ A1 ->
+     s_neq_stvar Ψ A2 ->
+     s_neq_stvar Ψ (typ_intersection A1 A2).
+
 (* defns J_d_sub *)
 Inductive d_sub : denv -> typ -> typ -> Prop :=    (* defn d_sub *)
  | d_sub__top : forall (Ψ:denv) (A:typ),
@@ -1392,15 +1417,13 @@ Inductive d_sub : denv -> typ -> typ -> Prop :=    (* defn d_sub *)
      d_sub Ψ A2 B2 ->
      d_sub Ψ (typ_arrow A1 A2) (typ_arrow B1 B2)
  | d_sub__all : forall (L:vars) (Ψ:denv) (A B:typ),
-      ( forall X , X \notin  L  -> s_in X  ( open_typ_wrt_typ A (typ_var_f X) )  )  ->
-      ( forall X , X \notin  L  -> s_in X  ( open_typ_wrt_typ B (typ_var_f X) )  )  ->
       ( forall X , X \notin  L  -> d_sub  ( X ~ dbind_stvar_empty  ++  Ψ )   ( open_typ_wrt_typ A (typ_var_f X) )   ( open_typ_wrt_typ B (typ_var_f X) )  )  ->
      d_sub Ψ (typ_all A) (typ_all B)
  | d_sub__alll : forall (L:vars) (Ψ:denv) (A B T:typ),
      neq_all B ->
      neq_intersection B ->
      neq_union B ->
-      ( forall X , X \notin  L  -> s_in X  ( open_typ_wrt_typ A (typ_var_f X) )  )  ->
+      ( forall X , X \notin  L  -> s_neq_stvar  ( X ~ dbind_tvar_empty  ++  Ψ )   ( open_typ_wrt_typ A (typ_var_f X) )  )  ->
      d_mono_typ Ψ T ->
      d_sub Ψ  (open_typ_wrt_typ  A   T )  B ->
      d_sub Ψ (typ_all A) B
@@ -1697,6 +1720,6 @@ Inductive a_wf_env : aenv -> Prop :=    (* defn a_wf_env *)
 
 
 (** infrastructure *)
-#[export] Hint Constructors s_in s_in_b neq_abs neq_all neq_intersection neq_union neq_bot d_wf_typ d_wf_exp d_wf_body d_wf_tenv d_wf_env d_mono_typ d_wf_conts d_wf_contd d_wf_work d_wf_twl d_wf_wl d_sub a_wf_typ a_mono_typ a_wf_exp a_wf_body a_wf_conts a_wf_contd a_wf_work a_wf_wwl a_wf_twl a_wf_wl a_wf_env lc_typ lc_exp lc_body lc_contd lc_conts lc_dbind lc_abind lc_work lc_aworklist lc_dworklist : core.
+#[export] Hint Constructors s_in s_in_b neq_abs neq_all neq_intersection neq_union neq_bot d_wf_typ d_wf_exp d_wf_body d_wf_tenv d_wf_env d_mono_typ d_wf_conts d_wf_contd d_wf_work d_wf_twl d_wf_wl s_neq_stvar d_sub a_wf_typ a_mono_typ a_wf_exp a_wf_body a_wf_conts a_wf_contd a_wf_work a_wf_wwl a_wf_twl a_wf_wl a_wf_env lc_typ lc_exp lc_body lc_contd lc_conts lc_dbind lc_abind lc_work lc_aworklist lc_dworklist : core.
 
 
